meeting work

test.thy
@@ -18,10 +18,6 @@ type_synonym '\<alpha> printer = "'\<alpha> \<Rightarrow> string option"
 
 type_synonym '\<alpha> bidef = "('\<alpha> parser \<times> '\<alpha> printer) option"
 
-(*WF should also include Inl \<Rightarrow> Inl and Inr \<Rightarrow> Inr*)
-type_synonym 'a bd = "(string + 'a) \<Rightarrow> ((('a \<times> string) option) + string option) option"
-
-
 abbreviation "option_lub \<equiv> flat_lub None"
 
 definition "bidef_ord = fun_ord option_ord"
@@ -57,12 +53,147 @@ definition return :: "'a \<Rightarrow> 'a bidef" where
 
 definition if_then_else :: "'\<alpha> bidef \<Rightarrow> ('\<alpha> \<Rightarrow> '\<beta> bidef) \<Rightarrow> '\<gamma> bidef \<Rightarrow> ('\<beta> \<Rightarrow> '\<alpha>) \<Rightarrow> ('\<beta> + '\<gamma>) bidef" where
   "if_then_else a a2b c b2a = ( do {
-      p_a \<leftarrow> a;
-      
+      p_a \<leftarrow> a; \<comment> \<open>Not sure what this means, we are supposed to create a bidef in this monad, where None means nonterm\<close>
       
       undefined
-
 })"
+
+
+\<comment> \<open>IDEA: We let the bidef be one function\<close>
+(*WF should also include Inl \<Rightarrow> Inl and Inr \<Rightarrow> Inr in wf*)
+type_synonym 'a bd_aux = "(string + 'a) \<Rightarrow> ((('a \<times> string)) + string) option"
+
+
+definition parse_aux :: "'a bd_aux \<Rightarrow> 'a parser" where
+  "parse_aux bd_aux s = map_option projl (bd_aux (Inl s))"
+
+definition print_aux :: "'a bd_aux \<Rightarrow> 'a printer" where
+  "print_aux bd_aux s = map_option projr (bd_aux (Inr s))"
+
+fun bdc_aux :: "('a parser) \<Rightarrow> ('a printer) \<Rightarrow> 'a bd_aux" where
+  "bdc_aux parser printer (Inl s) = map_option Inl (parser s)"
+| "bdc_aux parser printer (Inr t) = map_option Inr (printer t)"
+
+lemma bdc_aux_def:
+  "bdc_aux parser printer = (\<lambda> Inl s \<Rightarrow> map_option Inl (parser s) | Inr t \<Rightarrow> map_option Inr (printer t))"
+  by (auto simp add: fun_eq_iff split: sum.splits)
+
+lemma pp_bdc:
+  "parse_aux (bdc_aux p pr) = p"
+  "print_aux (bdc_aux p pr) = pr"
+  unfolding parse_aux_def print_aux_def bdc_aux_def
+  by (auto simp add: fun_eq_iff map_option.compositionality map_option.identity comp_def split: sum.splits)
+
+definition wf_bd_aux :: "'a bd_aux \<Rightarrow> bool" where
+  "wf_bd_aux bd_aux \<equiv> ( \<forall> s r. bd_aux (Inl s) = Some r \<longrightarrow> isl r) \<and> (\<forall> t r. (bd_aux (Inr t) = Some r \<longrightarrow> \<not>isl r))"
+
+lemma bd_aux_wf_bdc:
+  "wf_bd_aux (bdc_aux pa pr)"
+  unfolding bdc_aux_def wf_bd_aux_def
+  by auto
+
+lemma bdc_aux_tuple:
+  "wf_bd_aux bd \<Longrightarrow> wf_bd_aux bd' \<Longrightarrow> parse_aux bd = parse_aux bd' \<Longrightarrow> print_aux bd = print_aux bd' \<Longrightarrow> bd = bd'"
+  unfolding bdc_aux_def parse_aux_def print_aux_def wf_bd_aux_def
+  apply (clarsimp simp add: fun_eq_iff)
+  subgoal for x
+    apply (cases x)
+    subgoal for a
+      
+      apply( cases \<open>bd x\<close>; simp; cases \<open>bd' x\<close>; simp)
+        apply (auto  dest: spec[of _ a])
+      by (metis option.inject option.simps(9) sum.expand)
+    subgoal for b
+      apply( cases \<open>bd x\<close>; simp; cases \<open>bd' x\<close>; simp)
+        apply (auto  dest: spec[of _ b])
+      by (metis option.inject option.simps(9) sum.expand)
+    done
+  done
+
+
+lemma bdc_aux_all:
+  assumes "wf_bd_aux bd"
+  shows "bdc_aux (parse_aux bd) (print_aux bd) = bd"
+  by (simp add: assms bdc_aux_tuple bd_aux_wf_bdc pp_bdc(1) pp_bdc(2))
+
+typedef 'a bd = "Collect wf_bd_aux :: 'a bd_aux set"
+  apply (rule exI[of _ \<open>\<lambda>x. None\<close>])
+  by (simp add: wf_bd_aux_def)
+print_theorems
+
+setup_lifting type_definition_bd
+
+lift_definition parse :: "'a bd \<Rightarrow> 'a parser" is parse_aux . 
+lift_definition print :: "'a bd \<Rightarrow> 'a printer" is print_aux .
+lift_definition bdc :: "'a parser \<Rightarrow> 'a printer \<Rightarrow> 'a bd" is bdc_aux by (simp add: bd_aux_wf_bdc)
+
+lemma bdc'_tuple:
+  "parse bd = parse bd' \<Longrightarrow> print bd = print bd' \<Longrightarrow> bd = bd'"
+  apply transfer
+  by (simp add: bdc_aux_tuple)
+
+lemma bdc'_all:
+  shows "bdc (parse bd) (print bd) = bd"
+  apply transfer
+  by (simp add: bdc_aux_all)
+
+lifting_update bd.lifting
+lifting_forget bd.lifting
+
+definition bd_bottom :: "'a bd" where
+  "bd_bottom = bdc (\<lambda>x. None) (\<lambda>x. None)"
+
+
+
+interpretation bd:
+  partial_function_definitions "flat_ord bd_bottom" "flat_lub bd_bottom"
+  rewrites "flat_lub bd_bottom {} \<equiv> bd_bottom"
+by (rule flat_interpretation)(simp add: flat_lub_def)
+
+abbreviation "bd_ord \<equiv> flat_ord bd_bottom"
+abbreviation "mono_bd \<equiv> monotone (fun_ord bd_ord) bd_ord"
+(*
+lemma fixp_induct_bd:
+  fixes F :: "'c \<Rightarrow> 'c" and
+    U :: "'c \<Rightarrow> 'b \<Rightarrow> 'a bd" and
+    C :: "('b \<Rightarrow> 'a bd) \<Rightarrow> 'c" and
+    P :: "'b \<Rightarrow> 'a \<Rightarrow> bool"
+  assumes mono: "\<And>x. mono_bd (\<lambda>f. U (F (C f)) x)"
+  assumes eq: "f \<equiv> C (ccpo.fixp (fun_lub (flat_lub bd_bottom)) (fun_ord bd_ord) (\<lambda>f. U (F (C f))))"
+  assumes inverse2: "\<And>f. U (C f) = f"
+  assumes step: "\<And>f x y. (\<And>x y. U f x = Some y \<Longrightarrow> P x y) \<Longrightarrow> U (F f) x = Some y \<Longrightarrow> P x y"
+  assumes defined: "U f x = Some y"
+  shows "P x y"
+  using step defined bd.fixp_induct_uc[of U F C, OF mono eq inverse2 option_admissible]
+  unfolding fun_lub_def flat_lub_def by(auto 9 2)
+*)
+
+declaration \<open>Partial_Function.init "bd" \<^term>\<open>bd.fixp_fun\<close>
+  \<^term>\<open>bd.mono_body\<close> @{thm bd.fixp_rule_uc} @{thm bd.fixp_induct_uc}
+  (NONE)\<close> (*SOME @{thm fixp_induct_option}*)
+
+\<comment> \<open>Define basics here\<close>
+(*
+return, fail(bottom?)
+ite, bind (derive?), (derive) then, else, etc
+
+
+For partial function needs a parameter, add a unit/dummy parameter
+*)
+
+\<comment> \<open>problem here, the types are all wrong. a expects a str+'a, but we get a str+('a+'c)\<close>
+\<comment> \<open>This might be resolvable, but I'll have to think about it more.\<close>
+definition ite :: "'a bd_aux \<Rightarrow> ('a \<Rightarrow> 'b bd) \<Rightarrow> 'c bd_aux \<Rightarrow> ('b \<Rightarrow> 'a) \<Rightarrow> ('a + 'c) bd" where
+  "ite a a2b c b2a i = (
+      case i of
+        \<comment> \<open>parsing\<close>
+        Inl l \<Rightarrow> undefined
+        \<comment> \<open>printing 'a\<close>
+      | Inr (Inl rl) \<Rightarrow> undefined
+        \<comment> \<open>printing 'c\<close>
+      | Inr (Inr rr) \<Rightarrow> c rr
+
+)"
 
 
 end
